coqimp/framework/soundness/sep_tactic.v
@@ -26,41 +26,6 @@ Ltac destruct_state s :=
   destruct s as [ [ ?m [?r ?f] ] ?d ].
 
 (*+ Some tactic for Sep Proof +*)
-Fixpoint get_nth_asrt (a : asrt) (n : nat) : option asrt :=
-  match n with
-  | O => match a with
-        | p ** q => Some p
-        | _ => Some a
-        end
-  | S n' => match a with
-           | p ** q => get_nth_asrt q n'
-           | _ => None
-           end
-  end.
-
-Fixpoint remove_nth_asrt (a : asrt) (n : nat) : asrt :=
-  match n with
-  | O => match a with
-        | p ** q => q
-        | _ => Aemp
-        end
-  | S n' => match a with
-           | p ** q => p ** remove_nth_asrt q n'
-           | _ => a
-           end
-  end.
-
-Definition lift_nth_asrt (a : asrt) (n : nat) : asrt :=
-  match get_nth_asrt a n with
-  | Some p =>
-    match remove_nth_asrt a n with
-    | Aemp => p
-    | q => p ** q
-    end
-  | _ => a
-  end.
-
-(* test *)
 
 
 Theorem lift_assert_stable :
