coqimp/framework/soundness/wfcdhp_sound.v
@@ -1,0 +1,76 @@
+Require Import Coqlib.  
+Require Import Maps. 
+Require Import LibTactics.
+
+Require Import Integers.
+Open Scope Z_scope.  
+Import ListNotations.
+
+Set Asymmetric Patterns.
+   
+Require Import state. 
+Require Import language.
+
+Set Implicit Arguments.
+Unset Strict Implicit.
+         
+Require Import logic. 
+Require Import soundness.
+ 
+Require Import lemmas.
+
+Require Import inssound.
+
+Require Import Coq.Logic.FunctionalExtensionality.
+ 
+Open Scope nat.
+Open Scope code_scope.
+
+Ltac get_ins_diff_false :=
+  match goal with
+  | H1 : ?C ?pc = _, H2 : ?C ?pc = _ |- _ =>
+    rewrite H1 in H2; inversion H2;
+    tryfalse; subst
+  end.
+
+Lemma insSeq_rule_sound :
+  forall Spec Spec' p q I pc npc S C,
+    wf_seq Spec p I q -> LookupC C pc npc I ->
+    wf_cdhp Spec C Spec' -> cdhp_subst Spec Spec' -> S |= p ->
+    safety C S pc npc q 0.
+Proof.
+  cofix.
+
+  intros.
+  eapply safety_cons.
+
+  - (** Seq *)
+    intros.
+    inversion H0; subst; get_ins_diff_false.
+    inversion H; subst.
+    {
+      (* Normal *)
+      inversion H5; subst.
+      inversion H18; get_ins_diff_false.
+      clear H18.
+      eapply ins_rule_sound in H14; eauto.
+    }
+    
+  
+Theorem cdhp_rule_sound :
+  forall C Spec Spec',
+    wf_cdhp Spec C Spec' ->
+    cdhp_sound C Spec Spec'.
+Proof.
+  intros.
+  unfolds cdhp_sound.
+  intros.
+  unfolds wf_cdhp.
+  lets Hspec : H0. 
+  eapply H with (L := L) in Hspec; eauto.
+  simpljoin1. 
+  rename x into I.
+  eapply insSeq_rule_sound ; eauto.
+Qed.
+
+  
